\documentclass[../main.tex]{subfiles}

\pagestyle{main}
\renewcommand{\chaptermark}[1]{\markboth{\chaptername\ \thechapter}{}}
\setcounter{chapter}{11}

\begin{document}




\chapter{Derivatives}\label{sct:12}
\section{Journal}
\marginnote{3/30:}Throughout this sheet, we let $f:A\to\R$ be a real valued function with domain $A\subset\R$. We also now assume the domain $A\subset\R$ is open.
\begin{definition}\label{dfn:12.1}
    The \textbf{derivative} of $f$ at a point $a\in A$ is the number $f'(a)$ defined by the limit
    \begin{equation*}
        f'(a) = \lim_{h\to 0}\frac{f(a+h)-f(a)}{h}
    \end{equation*}
    provided that the limit on the right-hand side exists. If $f'(a)$ exists, we say that $f$ is \textbf{differentiable} (at $a$). If $f$ is differentiable at all points of its domain, we say that $f$ is \textbf{differentiable}. In this case, the values $f'(a)$ define a new function $f':A\to\R$ called the \textbf{derivative} (of $f$).
\end{definition}

\begin{remark}\label{rmk:12.2}
    If $A$ is not open, the limit in Definition \ref{dfn:12.1} may not exist. For example, if $f:[a,b]\to\R$, then we cannot define the derivative at the endpoints. For any $c$ in the domain of $f$, we define the \textbf{right-hand derivative} $f'_+(c)$ and the \textbf{left-hand derivative} $f'_-(c)$ by
    \begin{align*}
        f'_+(c) &= \lim_{h\to 0^+}\frac{f(c+h)-f(c)}{h}&
        f'_-(c) &= \lim_{h\to 0^-}\frac{f(c+h)-f(c)}{h}
    \end{align*}
    We say that $f$ is \textbf{differentiable} (on $[a,b]$) if $f$ is differentiable on $(a,b)$ and $f'_+(a)$ and $f'_-(b)$ exist.
\end{remark}

% Take out exercise in preamble!!!
\begin{lemma}\label{lem:12.3}
    Let $a\in\R$. Then
    \begin{equation*}
        \lim_{x\to a}f(x) = \lim_{h\to 0}f(a+h)
    \end{equation*}
    assuming that one of the two limits exists. (So if the limit on the left exists, so does the one on the right, and they are equal. Similarly, if the limit on the right exists, then so does the one on the left, and they are equal.)
    \begin{proof}
        Suppose first that $\lim_{x\to a}f(x)$ exists, and let it be equal to $L$. To prove that $\lim_{h\to 0}f(a+h)$ exists and that it equals $\lim_{x\to a}f(x)$, Definition \ref{dfn:11.1} tells us that it will suffice to show that for every $\epsilon>0$, there exists a $\delta>0$ such that if $(h+a)\in A$ and $0<|h-0|=|h|<\delta$, then $|f(a+h)-L|<\epsilon$. Let $\epsilon>0$ be arbitrary. Since $\lim_{x\to a}f(x)$ exists, Definition \ref{dfn:11.1} implies that there exists a $\delta>0$ such that if $x\in A$ and $0<|x-a|<\delta$, then $|f(x)-L|<\epsilon$. We will choose this $\delta$ to be our $\delta$. Now suppose that $h$ is any number satisfying both $(h+a)\in A$ and $0<|h|<\delta$; we seek to show that $|f(a+h)-L|<\epsilon$. Since $(h+a)\in A$, $h+a=x$ for some $x\in A$. It follows that $h=x-a$, meaning that $x$ is an object that is both an element of $A$ and that satisfies $0<|h|=|x-a|<\delta$, so we know that $|f(a+h)-L|=|f(x)-L|<\epsilon$, as desired.\par
        The proof is symmetric in the other direction.
    \end{proof}
\end{lemma}

\begin{theorem}\label{trm:12.4}
    Let $a\in\R$. Then $f$ is differentiable at $a$ if and only if $\lim_{x\to a}\frac{f(x)-f(a)}{x-a}$ exists. Moreover, if $f$ is differentiable at $a$, then the derivative of $f$ at $a$ is given by the limit
    \begin{equation*}
        f'(a) = \lim_{x\to a}\frac{f(x)-f(a)}{x-a}
    \end{equation*}
    \begin{proof}
        Suppose first that $f$ is differentiable at $a$. Then by Definition \ref{dfn:12.1}, $f'(a)$ exists. It follows that
        \begin{align*}
            f'(a) &= \lim_{h\to 0}\frac{f(a+h)-f(a)}{h}\tag*{Definition \ref{dfn:12.1}}\\
            &= \lim_{h\to 0}\frac{f(a+h)-f(a)}{(a+h)-a}\\
            &= \lim_{x\to a}\frac{f(x)-f(a)}{x-a}\tag*{Lemma \ref{lem:12.3}}
        \end{align*}
        Note that the substitution in the last step follows from using $\tilde{f}(x)=\frac{f(x)-f(a)}{x-a}$ as the "$f(x)$" function in Lemma \ref{lem:12.3}.\par
        The proof is symmetric in the reverse direction.
    \end{proof}
\end{theorem}

\begin{theorem}\label{trm:12.5}
    If $f$ is differentiable at $a$, then $f$ is continuous at $a$.
    \begin{proof}
        To prove that $f$ is continuous at $a$, Theorem \ref{trm:11.5} tells us that it will suffice to show that $\lim_{x\to a}f(x)=f(a)$. By Definition \ref{dfn:12.1}, the hypothesis implies that $f'(a)$ exists. Additionally, by Exercise \ref{exr:11.6}, $g(x)=x-a$ is continuous at $a$. Thus, by Theorem \ref{trm:11.5}, $\lim_{x\to a}g(x)$ exists (and equals $g(a)$). Consequently, knowing that both $\lim_{x\to a}\frac{f(x)-f(a)}{x-a}$ and $\lim_{x\to a}g(x)$ exist (the former by Theorem \ref{trm:12.4}), we have by Theorem \ref{trm:11.9} that the limit of their product exists and equals
        \begin{align*}
            \lim_{x\to a}\left( \frac{f(x)-f(a)}{x-a}\cdot(x-a) \right) = \lim_{x\to a}(f(x)-f(a))
        \end{align*}
        Moreover, since $g$ is continuous at $a$, $\lim_{x\to a}g(x)=g(a)=a-a=0$. Thus,
        \begin{align*}
            \lim_{x\to a}(f(x)-f(a)) &= \left( \lim_{x\to a}\frac{f(x)-f(a)}{x-a} \right)\left( \lim_{x\to a}(x-a) \right)\\
            &= \left( \lim_{x\to a}\frac{f(x)-f(a)}{x-a} \right)\cdot 0\\
            &= 0
        \end{align*}
        But then it follows by Theorem \ref{trm:11.9} if we consider $f(a)$ to be a constant function that
        \begin{align*}
            \lim_{x\to a}(f(x)-f(a))+f(a) &= 0+f(a)\\
            \lim_{x\to a}(f(x)-f(a)+f(a)) &= f(a)\\
            \lim_{x\to a}f(x) &= f(a)
        \end{align*}
        as desired.
    \end{proof}
\end{theorem}

\begin{exercise}\label{exr:12.6}
    Show that the converse of Theorem \ref{trm:12.5} is not true.
    \begin{proof}
        % Consider the absolute value function (Exercise \ref{exr:11.7}).

        The converse of Theorem \ref{trm:12.5} asserts that "if $f$ is continuous at $a$, then $f$ is differentiable at $a$." To falsify this statement, we will use the absolute value function $|x|$ as a counterexample. Let's begin.\par
        By Exercise \ref{exr:11.7}, $|x|$ is continuous. It follows by Theorem \ref{trm:9.10} that $|x|$ is continuous at 0. However, we can show that $|x|$ is not differentiable at 0.\par
        To do this, Definition \ref{dfn:12.1} and Theorem \ref{trm:12.4} tell us that it will suffice to verify that $\lim_{x\to 0}\frac{|x|-|0|}{x-0}=\lim_{x\to 0}\frac{|x|}{x}$ does not exist. Suppose for the sake of contradiction that $\lim_{x\to 0}\frac{|x|}{x}=L$. Then by Definition \ref{dfn:11.1}, for $\epsilon=1>0$, there exists a $\delta>0$ such that if $0<|x-0|=|x|<\delta$, then $|\frac{|x|}{x}-L|<1$. However, we can show that no such $\delta$ exists. Let $\delta>0$ be arbitrary. By Theorem \ref{trm:5.2}, there exists a number $x\in\R$ such that $0<x<\delta$. It follows by Definition \ref{dfn:8.4} and Exercise \ref{exr:8.5} that $0<|x|=|-x|<\delta$. Since both $x$ and $-x$ are in the appropriate range, we know that
        \begin{align*}
            \left| \frac{|x|}{x}-L \right| &= \left| \frac{x}{x}-L \right|&
                \left| \frac{|-x|}{-x}-L \right| &= \left| \frac{x}{-x}-L \right|\tag*{Definition \ref{dfn:8.4}}\\
            &= |1-L|&
                &= |-1-L|\tag*{Script \ref{sct:7}}\\
            &= |L-1|&
                &= |L+1|\tag*{Exercise \ref{exr:8.5}}\\
            &< 1&
                &< 1
        \end{align*}
        By consecutive applications of the lemma from Exercise \ref{exr:8.9}, it follows that
        \begin{align*}
            -1 &< L-1 < 1&
                -1 &< L+1 < 1\\
            0 &< L < 2&
                -2 &< L < 0
        \end{align*}
        But this implies that $L<0$ and $L>0$, a contradiction.
    \end{proof}
\end{exercise}

\begin{exercise}\label{exr:12.7}
    Show that for all $n\in\N$,
    \begin{equation*}
        x^n-a^n = (x-a)\left( x^{n-1}+ax^{n-2}+a^2x^{n-3}+\cdots+a^{n-2}x+a^{n-1} \right)
    \end{equation*}
    or equivalently,
    \begin{equation*}
        x^n-a^n = (x-a)\left( \sum_{i=0}^{n-1}x^{n-1-i}a^i \right)
    \end{equation*}
    \begin{proof}
        By simple algebra (see Script \ref{sct:7}), we have
        \begin{align*}
            (x-a)\left( \sum_{i=0}^{n-1}x^{n-1-i}a^i \right) &= \sum_{i=0}^{n-1}(x-a)x^{n-1-i}a^i\\
            &= \sum_{i=0}^{n-1}\left( x^{n-i}a^i-x^{n-1-i}a^{i+1} \right)\\
            &= x^n+\sum_{i=1}^{n-1}x^{n-i}a^i-\sum_{i=0}^{n-2}x^{n-1-i}a^{i+1}-a^n\\
            &= x^n+\sum_{i=1}^{n-1}x^{n-i}a^i-\sum_{i=0+1}^{n-2+1}x^{n-1-(i-1)}a^{(i-1)+1}-a^n\\
            &= x^n+\sum_{i=1}^{n-1}x^{n-i}a^i-\sum_{i=1}^{n-1}x^{n-i}a^i-a^n\\
            &= x^n-a^n
        \end{align*}
    \end{proof}
\end{exercise}

\begin{exercise}\label{exr:12.8}\leavevmode
    \begin{enumerate}[label={(\alph*)}]
        \item Let $n\in\N$. Suppose $f:\R\to\R$ is given by $f(x)=x^n$. Use Exercise \ref{exr:12.7} to prove that $f'(a)=na^{n-1}$ for all $a\in\R$.
        \begin{proof}
            To prove that $f'(a)=na^{n-1}$ for all $a\in\R$, Theorem \ref{trm:12.4} tell us that it will suffice to show that $\lim_{x\to a}\frac{f(x)-f(a)}{x-a}=na^{n-1}$ for all $a\in\R$. Let $a$ be an arbitrary element of $\R$. By Corollary \ref{cly:11.12}, the polynomial $\sum_{i=0}^{n-1}x^{n-1-i}a^i$ is continuous. Thus, by Theorem \ref{trm:9.10}, it is continuous at $a$. It follows by Theorem \ref{trm:11.5} that $\lim_{x\to a}\sum_{i=0}^{n-1}x^{n-1-i}a^i=\sum_{i=0}^{n-1}a^{n-1-i}a^i$. Therefore,
            \begin{align*}
                na^{n-1} &= \underbrace{a^{n-1}+\cdots+a^{n-1}}_{n\text{ times}}\\
                &= \sum_{i=0}^{n-1}a^{n-1}\\
                &= \sum_{i=1}^{n-1}a^{n-1-i}a^i\\
                &= \lim_{x\to a}\sum_{i=0}^{n-1}x^{n-1-i}a^i\\
                &= \lim_{x\to a}\frac{x-a}{x-a}\cdot\sum_{i=0}^{n-1}x^{n-1-i}a^i
                \intertext{Note that we can make the above change because $\frac{x-a}{x-a}=1$ for all $x$ satisfying $0<|x-a|<\delta$, whatever $\delta$ may be.}
                &= \lim_{x\to a}\frac{x^n-a^n}{x-a}\tag*{Exercise \ref{exr:12.7}}\\
                &= \lim_{x\to a}\frac{f(x)-f(a)}{x-a}\\
                &= f'(a)\tag*{Theorem \ref{trm:12.4}}
            \end{align*}
            as desired.
        \end{proof}
        \item Let $k\in\R$. Prove that if $f:\R\to\R$ is given by $f(x)=k$, then $f'(a)=0$ for all $a\in\R$.
        \begin{proof}
            To prove that $f'(a)=0$ for all $a\in\R$, Definition \ref{dfn:12.1} tells us that it will suffice to show that $\lim_{h\to 0}\frac{f(a+h)-f(a)}{h}=0$ for all $a\in\R$. Let $a$ be an arbitrary element of $\R$. By Exercise \ref{exr:11.6}, the function $g(x)=0$ is continuous. Thus, by Theorem \ref{trm:9.10}, it is continuous at $a$. It follows by Theorem \ref{trm:11.5} that $\lim_{h\to 0}g(h)=g(0)=0$. Therefore,
            \begin{align*}
                0 &= \lim_{h\to 0}g(h)\\
                &= \lim_{h\to 0}0\\
                &= \lim_{h\to 0}\frac{h}{h}\cdot 0
                \intertext{Note that we can make the above change for the same reason as part (a).}
                &- \lim_{h\to 0}\frac{0}{h}\\
                &= \lim_{h\to 0}\frac{k-k}{h}\\
                &= \lim_{h\to 0}\frac{f(a+h)-f(a)}{h}
            \end{align*}
            as desired.
        \end{proof}
    \end{enumerate}
\end{exercise}

\begin{exercise}\label{exr:12.9}
    Suppose that $f:A\to\R$ and $g:A\to\R$ are differentiable at $a\in A$.
    \begin{enumerate}[label={(\alph*)}]
        \item Prove that $f+g$ is differentiable at $a$ and compute $(f+g)'(a)$ in terms of $f'(a)$ and $g'(a)$.
        \begin{proof}
            To prove that $f+g$ is differentiable at $a$, Definition \ref{dfn:12.1} tells us that it will suffice to show $\lim_{h\to 0}\frac{(f+g)(a+h)-(f+g)(a)}{h}$ exists. Since $f,g$ are differentiable at $a$, we know by Definition \ref{dfn:12.1} that $\lim_{h\to 0}\frac{f(a+h)-f(a)}{h}$ and $\lim_{h\to 0}\frac{g(a+h)-g(a)}{h}$ exist. Thus, by Theorem \ref{trm:11.9} the limit of their sum exists and equals
            \begin{align*}
                \lim_{h\to 0}\left( \frac{f(a+h)-f(a)}{h}+\frac{g(a+h)-g(a)}{h} \right) &= \lim_{h\to 0}\frac{f(a+h)+g(a+h)-f(a)-g(a)}{h}\\
                &= \lim_{h\to 0}\frac{(f+g)(a+h)-(f+g)(a)}{h}
            \end{align*}
            as desired. Having established that $\lim_{h\to 0}\frac{(f+g)(a+h)-(f+g)(a)}{h}$ exists, $(f+g)'(a)$ can be computed in terms of $f'(a)$ and $g'(a)$ with the following algebra.
            \begin{align*}
                (f+g)'(a) &= \lim_{h\to 0}\frac{(f+g)(a+h)-(f+g)(a)}{h}\tag*{Definition \ref{dfn:12.1}}\\
                &= \lim_{h\to 0}\left( \frac{f(a+h)-f(a)}{h}+\frac{g(a+h)-g(a)}{h} \right)\\
                &= \lim_{h\to 0}\frac{f(a+h)-f(a)}{h}+\lim_{h\to 0}\frac{g(a+h)-g(a)}{h}\tag*{Theorem \ref{trm:11.9}}\\
                &= f'(a)+g'(a)\tag*{Definition \ref{dfn:12.1}}
            \end{align*}
        \end{proof}
        \item Prove that $fg$ is differentiable and compute $(fg)'(a)$ in terms of $f(a)$, $g(a)$, $f'(a)$, and $g'(a)$.
        \begin{proof}
            To prove that $fg$ is differentiable at $a$, Definition \ref{dfn:12.1} tells us that it will suffice to show $\lim_{h\to 0}\frac{(fg)(a+h)-(fg)(a)}{h}$ exists. Since $f,g$ are differentiable at $a$, we know by Definition \ref{dfn:12.1} that $\lim_{h\to 0}\frac{f(a+h)-f(a)}{h}$ and $\lim_{h\to 0}\frac{g(a+h)-g(a)}{h}$ exist. For the same reason, we know by Theorem \ref{trm:12.5} that $g$ is continuous, i.e., continuous at $a$ by Theorem \ref{trm:9.10}. Consequently, by Theorem \ref{trm:11.5}, $\lim_{x\to a}g(x)$ exists (and equals $g(a)$). Note that the preceding limit is equal to $\lim_{h\to 0}g(a+h)$ by Lemma \ref{lem:12.3}. Lastly, we have by Exercise \ref{exr:11.6} that the constant function $f(a)$ is continuous at 0. Consequently, by Theorem \ref{trm:11.5}, $\lim_{h\to 0}f(a)$ exists (and equals $f(a)$). Combining all of these results, consecutive applications of Theorem \ref{trm:11.9} assert that the limits
            \begin{align*}
                \lim_{h\to 0}g(a+h)\cdot\frac{f(a+h)-f(a)}{h}&&
                \lim_{h\to 0}f(a)\cdot\frac{g(a+h)-g(a)}{h}
            \end{align*}
            exist. Furthermore, it asserts that the limit of their sum exists and equals
            \begin{align*}
                \lim_{h\to 0}\left( g(a+h)\cdot\frac{f(a+h)-f(a)}{h}+f(a)\cdot\frac{g(a+h)-g(a)}{h} \right)\\
                &\hspace{-5cm}= \lim_{h\to 0}\frac{g(a+h)(f(a+h)-f(a))+f(a)(g(a+h)-g(a))}{h}\\
                &\hspace{-5cm}= \lim_{h\to 0}\frac{f(a+h)g(a+h)-f(a)g(a+h)+f(a)g(a+h)-f(a)g(a)}{h}\\
                &\hspace{-5cm}= \lim_{h\to 0}\frac{f(a+h)g(a+h)-f(a)g(a)}{h}\\
                &\hspace{-5cm}= \lim_{h\to 0}\frac{(fg)(a+h)-(fg)(a)}{h}
            \end{align*}
            as desired. Having established that $\lim_{h\to 0}\frac{(fg)(a+h)-(fg)(a)}{h}$ exists, $(fg)'(a)$ can be computed in terms of $f(a)$, $g(a)$, $f'(a)$, and $g'(a)$ with the following algebra.
            \begin{align*}
                (fg)'(a) &= \lim_{h\to 0}\frac{(fg)(a+h)-(fg)(a)}{h}\tag*{Definition \ref{dfn:12.1}}\\
                &= \lim_{h\to 0}\left( g(a+h)\cdot\frac{f(a+h)-f(a)}{h}+f(a)\cdot\frac{g(a+h)-g(a)}{h} \right)\\
                &= \lim_{h\to 0}g(a+h)\cdot\lim_{h\to 0}\frac{f(a+h)-f(a)}{h}+\lim_{h\to 0}f(a)\cdot\lim_{h\to 0}\frac{g(a+h)-g(a)}{h}\tag*{Theorem \ref{trm:11.9}}\\
                &= g(a)f'(a)+f(a)g'(a)
            \end{align*}
        \end{proof}
        \item Prove that $\frac{1}{g}$ is differentiable at $a$ (under an appropriate assumption) and compute $(\frac{1}{g})'(a)$ in terms of $g'(a)$ and $g(a)$. What assumption do you need to make?
        \begin{proof}
            Assume, in addition to the fact that $g:A\to\R$ is differentiable at $a\in A$, that $g(a)\neq 0$.\par
            To prove that $\frac{1}{g}$ is differentiable at $a$, Definition \ref{dfn:12.1} tells us that it will suffice to show $\lim_{h\to 0}\frac{(\frac{1}{g})(a+h)-(\frac{1}{g})(a)}{h}$ exists. Since $g$ is differentiable at $a$, we know by Definition \ref{dfn:12.1} that $\lim_{h\to 0}\frac{g(a+h)-g(a)}{h}$ exists. For the same reason, we know by Theorem \ref{trm:12.5} that $g$ is continuous, i.e., continuous at $a$ by Theorem \ref{trm:9.10}. Consequently, by Theorem \ref{trm:11.5}, $\lim_{x\to a}g(x)$ exists (and equals $g(a)$). It follows by Lemma \ref{lem:12.3} that the preceding limit is equal to $\lim_{h\to 0}g(a+h)$. Thus, since it is also equal to $g(a)\neq 0$, we have by Theorem \ref{trm:11.9} that $\lim_{h\to 0}\frac{1}{g}(a+h)$ exists (and equals $\frac{1}{g(a)}$). Lastly, we have by Exercise \ref{exr:11.6} that the constant function $-\frac{1}{g(a)}$ is continuous at 0. Consequently, by Theorem \ref{trm:11.5}, $\lim_{h\to 0}-\frac{1}{g(a)}$ exists (and equals $-\frac{1}{g(a)}$). Combining this with the previous result, Theorem \ref{trm:11.9} asserts that the limit $\lim_{h\to 0}-\frac{1}{g(a+h)g(a)}$ exists (and equals $-\frac{1}{g(a)^2}$). Furthermore, it asserts that the limit of its product with $\lim_{h\to 0}\frac{(\frac{1}{g})(a+h)-(\frac{1}{g})(a)}{h}$ exists and equals
            \begin{align*}
                \lim_{h\to 0}-\frac{1}{g(a+h)g(a)}\cdot\frac{g(a+h)-g(a)}{h} &= \lim_{h\to 0}\frac{\frac{g(a)-g(a+h)}{g(a+h)g(a)}}{h}\\
                &= \lim_{h\to 0}\frac{\frac{1}{g(a+h)}-\frac{1}{g(a)}}{h}\\
                &= \lim_{h\to 0}\frac{(\frac{1}{g})(a+h)-(\frac{1}{g})(a)}{h}
            \end{align*}
            as desired. Having established that $\lim_{h\to 0}\frac{(\frac{1}{g})(a+h)-(\frac{1}{g})(a)}{h}$ exists, $(\frac{1}{g})'(a)$ can be computed in terms of $g(a)$ and $g'(a)$ with the following algebra.
            \begin{align*}
                \left( \frac{1}{g} \right)'(a) &= \lim_{h\to 0}\frac{\left( \frac{1}{g} \right)(a+h)-\left( \frac{1}{g} \right)(a)}{h}\tag*{Definition \ref{dfn:12.1}}\\
                &= \lim_{h\to 0}-\frac{1}{g(a+h)g(a)}\cdot\frac{g(a+h)-g(a)}{h}\\
                &= \lim_{h\to 0}-\frac{1}{g(a+h)g(a)}\cdot\lim_{h\to 0}\frac{g(a+h)-g(a)}{h}\tag*{Theorem \ref{trm:11.9}}\\
                &= -\frac{g'(a)}{g(a)^2}
            \end{align*}
        \end{proof}
        \item Prove that $\frac{f}{g}$ is differentiable at $a$ (under an appropriate assumption) and compute $(\frac{f}{g})'(a)$ in terms of $f(a)$, $g(a)$, $f'(a)$, and $g'(a)$. What assumption do you need to make?
        \begin{proof}
            Assume, in addition to the fact that $g:A\to\R$ is differentiable at $a\in A$, that $g(a)\neq 0$.\par
            It follows by part (c) that $\frac{1}{g}$ is differentiable at $a$, and then by part (b) that $f\cdot\frac{1}{g}=\frac{f}{g}$ is differentiable at $a$.\par
            Having established that $(\frac{f}{g})'(a)$ exists, it can be computed in terms of $f(a)$, $g(a)$, $f'(a)$, and $g'(a)$ with the following algebra.
            \begin{align*}
                \left( \frac{f}{g} \right)'(a) &= \left( f\cdot\frac{1}{g} \right)'(a)\\
                &= f(a)\left( \frac{1}{g} \right)'(a)+f'(a)\left( \frac{1}{g} \right)(a)\\
                &= f(a)\cdot -\frac{g'(a)}{g(a)^2}+\frac{f'(a)g(a)}{g(a)^2}\\
                &= \frac{f'(a)g(a)-f(a)g'(a)}{g(a)^2}
            \end{align*}
        \end{proof}
    \end{enumerate}
\end{exercise}




\end{document}